Weidenbach_Book/IsaSAT_Inner_Propagation.thy
@@ -1209,20 +1209,22 @@ definition update_blit_wl_heur_pre where
       simp flip: all_lits_alt_def2
       intro!: ASSERT_leI ASSERT_refine_right
       simp: vdom_m_update_subset)
-  subgoal for aa ab ac ad ae be af ag ah bf aj ak al am an bg ao bh ap aq ar bi at bz
-       ca ch cj ck cl cm cn cp cq cr cs cu y
-    apply (subgoal_tac \<open>vdom_m (all_atms cp (cq + cr + cs + cu))
-          (y(K := (y K)[ck := (ch, cm, cj)])) cp \<subseteq>
-        vdom_m (all_atms cp (cq + cr + cs + cu)) y cp\<close>)
+  subgoal for aa ab ac ad ae be af ag ah bf aj ak al am an bg ao bh ap aq ar bi at bl
+       bm bn bo bp bq br bs bt bu bv bw bx "by" bz ca cb ci cj ck cl cm cn co
+       cq cr cs ct cv y x
+    apply (subgoal_tac \<open>vdom_m (all_atms co (cq + cr + cs + ct))
+          (cv(K := (cv K)[ck := (ci, cm, cj)])) co \<subseteq>
+        vdom_m (all_atms co (cq + cr + cs + ct)) cv co\<close>)
     apply fast
     apply (rule vdom_m_update_subset')
     apply auto
     done
   subgoal for aa ab ac ad ae be af ag ah bf ai aj ak al am an bg ao bh ap aq ar bi at
-       bz ca ch ci cj ck cl cm cn co cp cq cr cs cu x
-    apply (subgoal_tac \<open>vdom_m (all_atms cn (cp + cq + cr + cs))
-         (cu(K := (cu K)[cj := (ch, cl, ci)])) cn \<subseteq>
-        vdom_m (all_atms cn (cp + cq + cr + cs)) cu cn\<close>)
+       bl bm bn bo bp bq br bs bt bu bv bw bx "by" bz ca cb ci cj ck cl cm cn
+       co cp cq cr cs ct cv x
+    apply (subgoal_tac \<open>vdom_m (all_atms co (cq + cr + cs + ct))
+         (cv(K := (cv K)[ck := (ci, cm, cj)])) co \<subseteq>
+        vdom_m (all_atms co (cq + cr + cs + ct)) cv co\<close>)
     apply fast
     apply (rule vdom_m_update_subset')
     apply auto
